Prefix: : <http://purl.net/dol/1.0/rdf#>
Prefix: dc: <http://purl.org/dc/elements/1.1/>
Prefix: dct: <http://purl.org/dc/terms/>
Prefix: owl: <http://www.w3.org/2002/07/owl#>
Prefix: rdf: <http://www.w3.org/1999/02/22-rdf-syntax-ns#>
Prefix: xml: <http://www.w3.org/XML/1998/namespace>
Prefix: xsd: <http://www.w3.org/2001/XMLSchema-datatypes#>
Prefix: rdfs: <http://www.w3.org/2000/01/rdf-schema#>
Prefix: todo: <http://example.org/todo#>



Ontology: <http://purl.net/dol/1.0/rdf#>


Annotations: 
    owl:versionInfo "1.0",
    rdfs:comment "RDF serialization of DOL, implemented as an OWL ontology.  Actually some axioms that we would like to have go beyond OWL.",
    todo:task "When scaling this ontology implementation up to DOL, look below for annotations marked as 'beyond OWL'.  These things can be modeled in FOL."

AnnotationProperty: dct:creator

    
AnnotationProperty: strictlyStrongerThan

    
AnnotationProperty: propagatesToAdjoint

    Annotations: 
        rdfs:comment "The subject class denotes a kind of mapping that, if it holds for a translation, also holds for the adjoint projection.",
        rdfs:comment "This is just for informative purposes: Even though it probably does not go beyond OWL, it doesn't work for annotation properties in Protégé
Domain: owl:Class
Range: xsd:boolean"
    
    Annotations: 
        rdfs:comment "The subject class denotes a kind of mapping that, if it holds for a translation, also holds for the adjoint projection.",
        rdfs:comment "This is just for informative purposes: Even though it probably does not go beyond OWL, it doesn't work for annotation properties in Protégé
Domain: owl:Class
Range: xsd:boolean"
    
    
AnnotationProperty: todo:task

    
AnnotationProperty: dct:date

    
AnnotationProperty: rdfs:comment

    
AnnotationProperty: owl:versionInfo

    
AnnotationProperty: supportsEntityKind

    Annotations: 
        rdfs:comment "This is just for informative purposes: Even though it probably does not go beyond OWL, it doesn't work for annotation properties in Protégé
Domain: OntologyLanguage
Range: owl:Class that rdfs:subClassOf value Entity"
    
    Annotations: 
        rdfs:comment "This is just for informative purposes: Even though it probably does not go beyond OWL, it doesn't work for annotation properties in Protégé
Domain: OntologyLanguage
Range: owl:Class that rdfs:subClassOf value Entity"
    
    
AnnotationProperty: entityKindIn

    Annotations: 
        rdfs:comment "This is just for informative purposes: It doesn't work for annotation properties
InverseOf: supportsEntityKind"
    
    Annotations: 
        rdfs:comment "This is just for informative purposes: It doesn't work for annotation properties
InverseOf: supportsEntityKind"
    
    
AnnotationProperty: reifiedBy

    Annotations: 
        rdfs:comment "The subject property is reified by the object class.",
        rdfs:comment "This is just for informative purposes: It doesn't work for annotation properties
InverseOf: reifies"
    
    Annotations: 
        rdfs:comment "The subject property is reified by the object class.",
        rdfs:comment "This is just for informative purposes: It doesn't work for annotation properties
InverseOf: reifies"
    
    
AnnotationProperty: dct:source

    
AnnotationProperty: reifies

    Annotations: 
        rdfs:comment "The subject class reifies the object property.",
        rdfs:comment "This is just for informative purposes: Even though it probably does not go beyond OWL, it doesn't work for annotation properties in Protégé
Domain: owl:Class
Range: owl:ObjectProperty"
    
    Annotations: 
        rdfs:comment "The subject class reifies the object property.",
        rdfs:comment "This is just for informative purposes: Even though it probably does not go beyond OWL, it doesn't work for annotation properties in Protégé
Domain: owl:Class
Range: owl:ObjectProperty"
    
    
AnnotationProperty: todo:question

    
Datatype: xsd:string

    
Datatype: xsd:date

    
Datatype: rdf:PlainLiteral

    
Datatype: xsd:boolean

    
ObjectProperty: embeddableInto

    Annotations: 
        rdfs:comment "The subject is embeddable into the object logic."
    
    SubPropertyOf: 
        translatableTo,
        exactlyMappableTo,
        modelBijectivelyMappableTo,
        mappableToLogic
    
    Characteristics: 
        Transitive
    
    
ObjectProperty: impliedExtensionOf

    Annotations: 
        strictlyStrongerThan <http://purl.net/dol/1.0/rdf#definitionallyExtends>
    
    SubPropertyOf: 
        definitionallyExtends
    
    
ObjectProperty: ontologyIn

    InverseOf: 
        hasOntology
    
    
ObjectProperty: conservativelyExtends

    Annotations: 
        dct:source "This synonym is inspired by CASL."
    
    EquivalentTo: 
        modelTheoreticallyConservativelyExtends
    
    
ObjectProperty: exactlyCorrespondingMapping

    Annotations: 
        rdfs:comment "The subject ontology language mapping exactly corresponds to the object logic mapping."
    
    Domain: 
        OntologyLanguageMapping
    
    Range: 
        LogicMapping
    
    
ObjectProperty: translatableFrom

    Annotations: 
        rdfs:comment "There is a translation from the object to the subject."
    
    SubPropertyOf: 
        mappableFrom
    
    InverseOf: 
        translatableTo
    
    
ObjectProperty: hasMember

    Domain: 
        DistributedOntology
    
    InverseOf: 
        memberOf
    
    
ObjectProperty: faithfullyMappableTo

    Annotations: 
        rdfs:comment "There is a faithful mapping from the subject to the object logic."
    
    SubPropertyOf: 
        mappableToLogic
    
    Characteristics: 
        Transitive
    
    
ObjectProperty: mappableToLogic

    Annotations: 
        rdfs:comment "There is a mapping from the subject logic to the object logic."
    
    SubPropertyOf: 
        mappableTo
    
    Characteristics: 
        Transitive
    
    InverseOf: 
        mappableFromLogic
    
    
ObjectProperty: extends

    Annotations: 
        
            Annotations: dct:creator "Christoph Lange", 
                         dct:date "2011-12-04"^^xsd:date
        todo:question "While the abstract and text syntaxes of DOL attach the 'kind of extension' to _one_ ontology, the semantics (CASL reference section 5.2.5) rather suggests that this is a relation between _two_ ontologies (which may or may not be given explicitly in the syntax).  Is it, therefore, OK, to model it like this in RDF?  Maybe we should also provide a semantically equivalent alternative that is more intuitive wrt. the syntax?"
    
    Domain: 
        Ontology
    
    Range: 
        Ontology
    
    
ObjectProperty: weaklyExactlyMappableTo

    Annotations: 
        rdfs:comment "There is a weakly exact mapping from the subject to the object logic."
    
    SubPropertyOf: 
        mappableToLogic
    
    Characteristics: 
        Transitive
    
    
ObjectProperty: subLanguageOf

    Annotations: 
        rdfs:comment "The subject is a sublanguage of the object ontology language.  Supported logics are shared along the inverse of this property.",
        
            Annotations: dct:creator "Christoph Lange", 
                         dct:date "2012-04-17"^^xsd:date
        todo:question "Do we need both subLanguageOf and profileOf?  Intuitively I do think so, and I think it's reasonable to distinguish them via their properties wrt. logic/serialization propagation."
    
    SubPropertyOf: 
        translatableTo,
        mappableToLanguage
    
    Characteristics: 
        Transitive
    
    
ObjectProperty: specifiesSemanticsOf

    InverseOf: 
        supportsLogic
    
    
ObjectProperty: translatableTo

    Annotations: 
        rdfs:comment "There is a translation from the subject to the object."
    
    SubPropertyOf: 
        mappableTo
    
    Characteristics: 
        Transitive
    
    InverseOf: 
        translatableFrom
    
    
ObjectProperty: mapsFrom

    Annotations: 
        rdfs:comment "The subject mapping maps from the object into something of the same type as the object.  (Enforcing the latter constraint goes beyond OWL.)"
    
    Characteristics: 
        Functional
    
    Domain: 
        Mapping
    
    InverseOf: 
        sourceOfMapping
    
    
ObjectProperty: exactlyMappableTo

    Annotations: 
        rdfs:comment "There is an exact mapping from the subject to the object logic."
    
    SubPropertyOf: 
        weaklyExactlyMappableTo
    
    Characteristics: 
        Transitive
    
    
ObjectProperty: language

    Annotations: 
        rdfs:comment "The reasoners in Protégé don't like us to say the following.  Together with the SubPropertyChain specified for supportsSerialization it would go beyond OWL DL anyway.
SubPropertyChain: serialization o serializes",
        rdfs:comment "the language of an ontology"
    
    Characteristics: 
        Functional
    
    Domain: 
        Ontology
    
    Range: 
        OntologyLanguage
    
    
ObjectProperty: modelBijectivelyMappableTo

    Annotations: 
        
            Annotations: dct:creator "Christoph Lange", 
                         dct:date "2012-04-17"^^xsd:date
        todo:question "Do we have a better idea for naming this?  Maybe mappableToWithBijectiveModels?",
        rdfs:comment "There is a model-bijective mapping from the subject to the object logic."
    
    SubPropertyOf: 
        modelExpansivelyMappableTo,
        weaklyExactlyMappableTo
    
    Characteristics: 
        Transitive
    
    
ObjectProperty: linkIn

    InverseOf: 
        hasLink
    
    
ObjectProperty: hasOntology

    Annotations: 
        rdfs:comment "The subject is a distributed ontology, in which the object is a participating heterogeneous ontology."
    
    SubPropertyOf: 
        hasMember
    
    Range: 
        Ontology
    
    InverseOf: 
        ontologyIn
    
    
ObjectProperty: projectableTo

    Annotations: 
        rdfs:comment "There is a projection from the subject to the object."
    
    SubPropertyOf: 
        mappableTo
    
    Characteristics: 
        Transitive
    
    InverseOf: 
        projectableFrom
    
    
ObjectProperty: target

    Annotations: 
        rdfs:comment "the target ontology of a link"
    
    Characteristics: 
        Functional
    
    Domain: 
        Link
    
    Range: 
        Ontology
    
    
ObjectProperty: source

    Annotations: 
        rdfs:comment "the source ontology of a link"
    
    Characteristics: 
        Functional
    
    Domain: 
        Link
    
    Range: 
        Ontology
    
    
ObjectProperty: exactLogicalExpressivity

    Annotations: 
        rdfs:comment "The subject ontology language has exactly the expressivity of the object logic."
    
    SubPropertyOf: 
        supportsLogic
    
    
ObjectProperty: serializes

    InverseOf: 
        supportsSerialization
    
    
ObjectProperty: monomorphicallyExtends

    Annotations: 
        strictlyStrongerThan <http://purl.net/dol/1.0/rdf#modelTheoreticallyConservativelyExtends>
    
    SubPropertyOf: 
        modelTheoreticallyConservativelyExtends
    
    
ObjectProperty: hasInterpretation

    Annotations: 
        rdfs:comment "The subject is a distributed ontology, in which the object is an interpretation between two participating ontologies."
    
    SubPropertyOf: 
        hasLink
    
    Range: 
        Interpretation
    
    InverseOf: 
        interpretationIn
    
    
ObjectProperty: hasAlignment

    Annotations: 
        rdfs:comment "The subject is a distributed ontology, in which the object is an alignment between two participating ontologies."
    
    SubPropertyOf: 
        hasLink
    
    Range: 
        Alignment
    
    InverseOf: 
        alignmentIn
    
    
ObjectProperty: memberOf

    InverseOf: 
        hasMember
    
    
ObjectProperty: modelTheoreticallyConservativelyExtends

    Annotations: 
        strictlyStrongerThan <http://purl.net/dol/1.0/rdf#consequenceTheoreticallyConservativelyExtends>
    
    SubPropertyOf: 
        consequenceTheoreticallyConservativelyExtends
    
    EquivalentTo: 
        conservativelyExtends
    
    
ObjectProperty: supportsLogic

    Annotations: 
        rdfs:comment "The semantics of [a subset of] the subject ontology language can be specified in terms of the object logic."
    
    SubPropertyChain: 
        
            Annotations: 
                         Annotations: dct:creator "Christoph Lange", 
                                     dct:date "2012-04-17"^^xsd:date
                                     
                                     todo:question "On the board we had 'inverse subLanguageOf o exactLogicalExpressivity', but I think we can be more general."
         inverse (subLanguageOf) o supportsLogic
    
    SubPropertyChain: 
        supportsLogic o  inverse (subLogicOf)
    
    Domain: 
        OntologyLanguage
    
    Range: 
        Logic
    
    InverseOf: 
        specifiesSemanticsOf
    
    
ObjectProperty: mappableToLanguage

    Annotations: 
        rdfs:comment "There is a mapping from the subject ontology language to the object ontology language."
    
    SubPropertyOf: 
        mappableTo
    
    Characteristics: 
        Transitive
    
    InverseOf: 
        mappableFromLanguage
    
    
ObjectProperty: alignmentIn

    InverseOf: 
        hasAlignment
    
    
ObjectProperty: sourceOfMapping

    InverseOf: 
        mapsFrom
    
    
ObjectProperty: mapsTo

    Annotations: 
        rdfs:comment "The subject mapping maps from something into the object (which is of the same type).  Enforcing the latter constraint goes beyond OWL."
    
    Characteristics: 
        Functional
    
    Domain: 
        Mapping
    
    
ObjectProperty: subLogicOf

    Annotations: 
        rdfs:comment "The subject is a sublogic of the object."
    
    SubPropertyOf: 
        embeddableInto
    
    SubPropertyChain: 
         inverse (exactLogicalExpressivity) o subLanguageOf o exactLogicalExpressivity
    
    Characteristics: 
        Transitive
    
    
ObjectProperty: interpretationIn

    InverseOf: 
        hasInterpretation
    
    
ObjectProperty: mappableFrom

    Annotations: 
        rdfs:comment "There is a mapping from the object to the subject."
    
    InverseOf: 
        mappableTo
    
    
ObjectProperty: compositionOf

    Annotations: 
        rdfs:comment "Range can't be specified in OWL DL",
        
            Annotations: dct:creator "Christoph Lange", 
                         dct:date "2012-04-30"^^xsd:date
        todo:question "I don't think we need subclasses for specific types of mappings, do we?",
        rdfs:comment "The subject mapping is the composition of the object list of mappings (list item 1 ∘ list item 2 ∘ … ∘ list item n).  All elements of the latter list must be instances of the same class as the subject.  (Enforcing the latter constraint goes beyond OWL.)"
    
    Domain: 
        Mapping
    
    
ObjectProperty: theoroidallyMappableTo

    Annotations: 
        rdfs:comment "There is a theoroidal mapping from the subject to the object logic."
    
    SubPropertyOf: 
        mappableToLogic
    
    Characteristics: 
        Transitive
    
    
ObjectProperty: logic

    Annotations: 
        
            Annotations: dct:creator "Christoph Lange", 
                         dct:date "2011-12-04"^^xsd:date
        todo:question "Inside a 'logic section' in the abstract syntax, there are also views.  Therefore, do we need another, analogous RDF property for 'the logic of a view'?",
        rdfs:comment "the logic in which an ontology is formalized"
    
    Characteristics: 
        Functional
    
    Domain: 
        Ontology
    
    Range: 
        Logic
    
    
ObjectProperty: modelExpansivelyMappableTo

    Annotations: 
        rdfs:comment "There is a model-expansive mapping from the subject to the object logic."
    
    SubPropertyOf: 
        faithfullyMappableTo
    
    Characteristics: 
        Transitive
    
    
ObjectProperty: mappableFromLogic

    Annotations: 
        rdfs:comment "There is a mapping from the object logic to the subject logic."
    
    InverseOf: 
        mappableToLogic
    
    
ObjectProperty: consequenceTheoreticallyConservativelyExtends

    SubPropertyOf: 
        extends
    
    
ObjectProperty: profileOf

    Annotations: 
        rdfs:comment "The subject is a profile of the object ontology language.  This is a stronger notion than just being a sublanguage.  Supported serializations are shared along this property."
    
    SubPropertyOf: 
        subLanguageOf
    
    
ObjectProperty: mappableFromLanguage

    Annotations: 
        rdfs:comment "There is a mapping from the object ontology language to the subject ontology language."
    
    InverseOf: 
        mappableToLanguage
    
    
ObjectProperty: serialization

    Annotations: 
        rdfs:comment "the serialization in which an ontology is written"
    
    Characteristics: 
        Functional
    
    Domain: 
        Ontology
    
    Range: 
        Serialization
    
    
ObjectProperty: mappableTo

    Annotations: 
        rdfs:comment "There is a mapping from the subject to the object."
    
    SubPropertyChain: 
        sourceOfMapping o mapsTo
    
    Characteristics: 
        Transitive
    
    InverseOf: 
        mappableFrom
    
    
ObjectProperty: hasLink

    Annotations: 
        rdfs:comment "The subject is a distributed ontology, in which the object is a link between two participating ontologies."
    
    SubPropertyOf: 
        hasMember
    
    Range: 
        Link
    
    InverseOf: 
        linkIn
    
    
ObjectProperty: definitionallyExtends

    Annotations: 
        strictlyStrongerThan <http://purl.net/dol/1.0/rdf#monomorphicallyExtends>
    
    SubPropertyOf: 
        monomorphicallyExtends
    
    
ObjectProperty: adjoint

    Domain: 
        Translation
    
    Range: 
        Projection
    
    
ObjectProperty: plainlyMappableTo

    Annotations: 
        rdfs:comment "There is a plain mapping from the subject to the object logic."
    
    SubPropertyOf: 
        theoroidallyMappableTo
    
    Characteristics: 
        Transitive
    
    
ObjectProperty: supportsSerialization

    Annotations: 
        rdfs:comment "The reasoners in Protégé don't like us to say the following.  Together with the SubPropertyChain specified for language it would go beyond OWL DL anyway.
SubPropertyChain: profileOf o supportsSerialization",
        rdfs:comment "Note that the serialization should be as specific as possible, i.e. one should not say that ``OWL can be serialized in XML'' and ``Common Logic can be serialized in XML'', but instead ``OWL can be serialized in OWL XML'' and ``Common Logic can be serialized in XCL'', taking into account that OWL XML and XCL are two different XML languages.",
        rdfs:comment "Ontologies in the subject ontology language can be serialized in the object serialization."
    
    Characteristics: 
        InverseFunctional
    
    Domain: 
        OntologyLanguage
    
    Range: 
        Serialization
    
    InverseOf: 
        serializes
    
    
ObjectProperty: projectableFrom

    Annotations: 
        rdfs:comment "There is a projection from the object to the subject."
    
    SubPropertyOf: 
        mappableFrom
    
    InverseOf: 
        projectableTo
    
    
DataProperty: mediaType

    Annotations: 
        rdfs:comment "the media type (MIME type) of a serialization"
    
    Characteristics: 
        Functional
    
    Domain: 
        Serialization
    
    Range: 
        xsd:string
    
    
DataProperty: prefFilenameExtension

    Annotations: 
        rdfs:comment "the preferred filename extension for a serialization"
    
    Characteristics: 
        Functional
    
    Domain: 
        Serialization
    
    Range: 
        xsd:string
    
    
DataProperty: altFilenameExtension

    Annotations: 
        rdfs:comment "an alternative filename extension for a serialization"
    
    Domain: 
        Serialization
    
    Range: 
        xsd:string
    
    
Class: owl:Thing

    
Class: WeaklyExactMapping

    Annotations: 
        propagatesToAdjoint "true"^^xsd:boolean,
        reifies <http://purl.net/dol/1.0/rdf#weaklyExactlyMappableTo>
    
    SubClassOf: 
        Mapping
    
    
Class: ExactMapping

    Annotations: 
        propagatesToAdjoint "true"^^xsd:boolean,
        reifies <http://purl.net/dol/1.0/rdf#exactlyMappableTo>
    
    SubClassOf: 
        WeaklyExactMapping
    
    
Class: DistributedOntology

    Annotations: 
        rdfs:comment "a distributed ontology"
    
    SubClassOf: 
        Ontology
    
    
Class: ModelExpansiveMapping

    Annotations: 
        propagatesToAdjoint "true"^^xsd:boolean,
        reifies <http://purl.net/dol/1.0/rdf#modelExpansivelyMappableTo>
    
    SubClassOf: 
        FaithfulMapping
    
    
Class: Translation

    Annotations: 
        rdfs:comment "a generic translation",
        reifies <http://purl.net/dol/1.0/rdf#translatableTo>
    
    SubClassOf: 
        Mapping
    
    DisjointWith: 
        Projection
    
    
Class: SubLogic

    Annotations: 
        rdfs:comment "'syntactic' embedding",
        reifies <http://purl.net/dol/1.0/rdf#subLogicOf>
    
    SubClassOf: 
        Embedding
    
    
Class: Sentence

    Annotations: 
        rdfs:comment "a sentence in an ontology"
    
    
Class: View

    Annotations: 
        rdfs:comment "a view (also called interpretation) between two heterogeneous ontologies in a distributed ontology"
    
    EquivalentTo: 
        Interpretation
    
    SubClassOf: 
        Link
    
    
Class: Embedding

    Annotations: 
        reifies <http://purl.net/dol/1.0/rdf#embeddableInto>
    
    SubClassOf: 
        ExactMapping,
        LogicMapping,
        Translation,
        ModelBijectiveMapping
    
    
Class: Ontology

    Annotations: 
        rdfs:comment "an ontology, distributed or basic"
    
    
Class: Interpretation

    EquivalentTo: 
        View
    
    DisjointWith: 
        Alignment
    
    
Class: OntologyLanguageMapping

    Annotations: 
        rdfs:comment "a mapping (translation or projection) between two ontology languages",
        propagatesToAdjoint "true"^^xsd:boolean
    
    SubClassOf: 
        Mapping
    
    DisjointWith: 
        LogicMapping
    
    
Class: Logic

    Annotations: 
        rdfs:comment "a logic that defines the semantics of an ontology language"
    
    
Class: TheoroidalMapping

    Annotations: 
        propagatesToAdjoint "true"^^xsd:boolean,
        reifies <http://purl.net/dol/1.0/rdf#theoroidallyMappableTo>,
        rdfs:comment "orthogonal to WeaklyExactMapping and FaithfulMapping"
    
    EquivalentTo: 
        Mapping
         and (not (PlainMapping))
    
    SubClassOf: 
        Mapping
    
    DisjointWith: 
        PlainMapping,
        
            Annotations: rdfs:comment "Protégé 4.2 doesn't like 'Class: Mapping DisjointUnionOf: PlainMapping, TheoroidalMapping', so we do it this way:"
        PlainMapping
    
    
Class: LogicMapping

    Annotations: 
        rdfs:comment "a mapping (translation or projection) between two logics",
        propagatesToAdjoint "true"^^xsd:boolean
    
    SubClassOf: 
        Mapping
    
    DisjointWith: 
        OntologyLanguageMapping
    
    
Class: Entity

    Annotations: 
        rdfs:comment "an entity in an ontology"
    
    
Class: Projection

    Annotations: 
        reifies <http://purl.net/dol/1.0/rdf#projectableTo>,
        rdfs:comment "a generic projection"
    
    SubClassOf: 
        Mapping
    
    DisjointWith: 
        Translation
    
    
Class: BasicOntology

    Annotations: 
        rdfs:comment "a basic ontology (in a single language, logic, and serialization)"
    
    SubClassOf: 
        Ontology
    
    
Class: FaithfulMapping

    Annotations: 
        propagatesToAdjoint "true"^^xsd:boolean,
        reifies <http://purl.net/dol/1.0/rdf#faithfullyMappableTo>
    
    SubClassOf: 
        Mapping
    
    
Class: Mapping

    Annotations: 
        reifies <http://purl.net/dol/1.0/rdf#mappableTo>,
        rdfs:comment "a generic mapping (translation or projection)"
    
    SubClassOf: 
        
            Annotations: rdfs:comment "Apparently one has to say 'owl:Thing' here; omitting it is legal by http://www.w3.org/TR/2009/NOTE-owl2-manchester-syntax-20091027/#Descriptions, but Protégé doesn't like it"
        (mapsFrom exactly 1 owl:Thing)
         and (mapsTo exactly 1 owl:Thing)
    
    
Class: DefaultMapping
    Annotations: 
        propagatesToAdjoint "true"^^xsd:boolean

    SubClassOf: 
        Mapping
    
    
Class: PlainMapping

    Annotations: 
        reifies <http://purl.net/dol/1.0/rdf#plainlyMappableTo>,
        propagatesToAdjoint "true"^^xsd:boolean
    
    SubClassOf: 
        Mapping
    
    DisjointWith: 
        TheoroidalMapping,
        
            Annotations: rdfs:comment "Protégé 4.2 doesn't like 'Class: Mapping DisjointUnionOf: PlainMapping, TheoroidalMapping', so we do it this way:"
        TheoroidalMapping
    
    
Class: Serialization

    Annotations: 
        rdfs:comment "a serialization of an ontology language"
    
    
Class: OntologyLanguage

    Annotations: 
        rdfs:comment "an ontology language"
    
    SubClassOf: 
        (supportsLogic some Logic)
         and (supportsSerialization some Serialization)
         and (supportsLogic only Logic)
         and (supportsSerialization only Serialization)
    
    
Class: Link

    Annotations: 
        rdfs:comment "a link between two heterogeneous ontologies in a distributed ontology"
    
    SubClassOf: 
        (source exactly 1 owl:Thing)
         and (target exactly 1 owl:Thing)
    
    
Class: ModelBijectiveMapping

    Annotations: 
        reifies <http://purl.net/dol/1.0/rdf#modelBijectivelyMappableTo>,
        propagatesToAdjoint "true"^^xsd:boolean
    
    SubClassOf: 
        WeaklyExactMapping,
        ModelExpansiveMapping
    
    
Class: Alignment

    Annotations: 
        rdfs:comment "an alignment between two heterogeneous ontologies in a distributed ontology"
    
    SubClassOf: 
        Link
    
    DisjointWith: 
        Interpretation
    
    
DisjointClasses: 
    Alignment,Logic,Mapping,Ontology,OntologyLanguage,Serialization

